James C - added continuation arguments to stack, b_assm, assm (not yet fixed conversions)

AssemblyLanguage.thy
@@ -8,32 +8,33 @@ datatype assembly =
 | JAssm "comparison set" code_label
 | PAssm
 
-type_synonym assembly_program = "code_label \<rightharpoonup> assembly list"
+type_synonym assembly_program = "code_label \<rightharpoonup> assembly list \<times> code_label"
 
-type_synonym assembly_state = "memory \<times> int option \<times> int \<times> assembly list \<times> output" 
-  (* \<mu>, a, d, \<pi>, \<omega> *)
+type_synonym assembly_state = "memory \<times> int option \<times> int \<times> assembly list \<times> code_label \<times> output" 
+  (* \<mu>, a, d, \<pi>, s, \<omega> *)
 
 fun eval_assembly :: "assembly_program \<Rightarrow> assembly_state \<Rightarrow> assembly_state option" where
-  "eval_assembly \<Pi> (\<mu>, a, d, [], \<omega>) = None"
-| "eval_assembly \<Pi> (\<mu>, a, d, AAssm x # \<pi>, \<omega>) = Some (\<mu>, Some x, d, \<pi>, \<omega>)"
-| "eval_assembly \<Pi> (\<mu>, Some a, d, CAssm dst cmp # \<pi>, \<omega>) = (
+  "eval_assembly \<Pi> (\<mu>, a, d, [], s, \<omega>) = (case \<Pi> s of 
+      Some (\<pi>', s') \<Rightarrow> Some (\<mu>, None, d, \<pi>', s', \<omega>)
+    | None \<Rightarrow> None)"
+| "eval_assembly \<Pi> (\<mu>, a, d, AAssm x # \<pi>, s, \<omega>) = Some (\<mu>, Some x, d, \<pi>, s, \<omega>)"
+| "eval_assembly \<Pi> (\<mu>, Some a, d, CAssm dst cmp # \<pi>, s, \<omega>) = (
     let n = compute cmp (\<mu> a) a d
     in Some (
       if M \<in> dst then \<mu>(a := n) else \<mu>, 
       Some (if A \<in> dst then n else a), 
       if D \<in> dst then n else d, 
-      \<pi>,
-      \<omega>))"
-| "eval_assembly \<Pi> (\<mu>, None, d, CAssm dst cmp # \<pi>, \<omega>) = None"
-| "eval_assembly \<Pi> (\<mu>, a, d, JAssm jmp s # \<pi>, \<omega>) = (
+      \<pi>, s, \<omega>))"
+| "eval_assembly \<Pi> (\<mu>, None, d, CAssm dst cmp # \<pi>, s, \<omega>) = None"
+| "eval_assembly \<Pi> (\<mu>, a, d, JAssm jmp s # \<pi>, s', \<omega>) = (
     if should_jump d jmp
     then case \<Pi> s of 
-        Some \<pi>' \<Rightarrow> Some (\<mu>, None, d, \<pi>', \<omega>)
+        Some (\<pi>', s'') \<Rightarrow> Some (\<mu>, None, d, \<pi>', s'', \<omega>)
       | None \<Rightarrow> None
-    else Some (\<mu>, None, d, \<pi>, \<omega>))"
-| "eval_assembly \<Pi> (\<mu>, a, d, PAssm # \<pi>, \<omega>) = Some (\<mu>, a, d, \<pi>, d # \<omega>)"
+    else Some (\<mu>, None, d, \<pi>, s', \<omega>))"
+| "eval_assembly \<Pi> (\<mu>, a, d, PAssm # \<pi>, s, \<omega>) = Some (\<mu>, a, d, \<pi>, s, d # \<omega>)"
 
 fun assembly_output :: "assembly_state \<Rightarrow> output" where
-  "assembly_output (\<mu>, a, d, \<pi>, \<omega>) = \<omega>"
+  "assembly_output (\<mu>, a, d, \<pi>, s, \<omega>) = \<omega>"
 
 end
