BranchingAssemblyLanguage.thy
@@ -9,32 +9,34 @@ datatype b_assembly =
 | JBAssm code_label
 | PBAssm
 
-type_synonym b_assembly_program = "code_label \<rightharpoonup> b_assembly list"
+type_synonym b_assembly_program = "code_label \<rightharpoonup> b_assembly list \<times> code_label"
 
-type_synonym b_assembly_state = "memory \<times> int option \<times> int \<times> b_assembly list \<times> output" 
-  (* \<mu>, a, d, \<pi>, \<omega> *)
+type_synonym b_assembly_state = "memory \<times> int option \<times> int \<times> b_assembly list \<times> code_label \<times> output" 
+  (* \<mu>, a, d, \<pi>, s, \<omega> *)
 
 fun eval_b_assembly :: "b_assembly_program \<Rightarrow> b_assembly_state \<Rightarrow> b_assembly_state option" where
-  "eval_b_assembly \<Pi> (\<mu>, a, d, [], \<omega>) = None"
-| "eval_b_assembly \<Pi> (\<mu>, a, d, ABAssm x # \<pi>, \<omega>) = Some (\<mu>, Some x, d, \<pi>, \<omega>)"
-| "eval_b_assembly \<Pi> (\<mu>, Some a, d, CBAssm dst cmp # \<pi>, \<omega>) = (
+  "eval_b_assembly \<Pi> (\<mu>, a, d, [], s, \<omega>) = (
+    case \<Pi> s of 
+      Some (\<pi>', s') \<Rightarrow> Some (\<mu>, a, d, \<pi>', s', \<omega>)
+    | None \<Rightarrow> None)"
+| "eval_b_assembly \<Pi> (\<mu>, a, d, ABAssm x # \<pi>, s, \<omega>) = Some (\<mu>, Some x, d, \<pi>, s, \<omega>)"
+| "eval_b_assembly \<Pi> (\<mu>, Some a, d, CBAssm dst cmp # \<pi>, s, \<omega>) = (
     let n = compute cmp (\<mu> a) a d
     in Some (
       if M \<in> dst then \<mu>(a := n) else \<mu>, 
       Some (if A \<in> dst then n else a), 
       if D \<in> dst then n else d, 
-      \<pi>, 
-      \<omega>))"
-| "eval_b_assembly \<Pi> (\<mu>, None, d, CBAssm dst cmp # \<pi>, \<omega>) = None"
-| "eval_b_assembly \<Pi> (\<mu>, a, d, IBAssm cmp \<pi>\<^sub>t \<pi>\<^sub>f # \<pi>, \<omega>) = 
-    Some (\<mu>, a, d, (if should_jump d cmp then \<pi>\<^sub>t else \<pi>\<^sub>f) @ \<pi>, \<omega>)"
-| "eval_b_assembly \<Pi> (\<mu>, a, d, JBAssm s # \<pi>, \<omega>) = (
+      \<pi>, s, \<omega>))"
+| "eval_b_assembly \<Pi> (\<mu>, None, d, CBAssm dst cmp # \<pi>, s, \<omega>) = None"
+| "eval_b_assembly \<Pi> (\<mu>, a, d, IBAssm cmp \<pi>\<^sub>t \<pi>\<^sub>f # \<pi>, s, \<omega>) = 
+    Some (\<mu>, a, d, (if should_jump d cmp then \<pi>\<^sub>t else \<pi>\<^sub>f) @ \<pi>, s, \<omega>)"
+| "eval_b_assembly \<Pi> (\<mu>, a, d, JBAssm s # \<pi>, s', \<omega>) = (
     case \<Pi> s of 
-      Some \<pi>' \<Rightarrow> Some (\<mu>, None, d, \<pi>', \<omega>)
+      Some (\<pi>', s'') \<Rightarrow> Some (\<mu>, None, d, \<pi>', s'', \<omega>)
     | None \<Rightarrow> None)"
-| "eval_b_assembly \<Pi> (\<mu>, a, d, PBAssm # \<pi>, \<omega>) = Some (\<mu>, a, d, \<pi>, d # \<omega>)"
+| "eval_b_assembly \<Pi> (\<mu>, a, d, PBAssm # \<pi>, s, \<omega>) = Some (\<mu>, a, d, \<pi>, s, d # \<omega>)"
 
 fun b_assembly_output :: "b_assembly_state \<Rightarrow> output" where
-  "b_assembly_output (\<mu>, a, d, \<pi>, \<omega>) = \<omega>"
+  "b_assembly_output (\<mu>, a, d, \<pi>, s, \<omega>) = \<omega>"
 
 end
