StackToAssembly.thy
@@ -77,7 +77,7 @@ primrec instruction_conv :: "stack_instruction \<Rightarrow> b_assembly list" wh
     CBAssm {M} (Decr M)]"
 
 definition program_convert :: "stack_program \<Rightarrow> b_assembly_program" where
-  "program_convert \<Pi> = map_option concat o map_option (map instruction_conv) o \<Pi>"
+  "program_convert \<Pi> = map_option (\<lambda>(\<pi>, s). (concat (map instruction_conv \<pi>), s)) o \<Pi>"
 
 primrec stack_to_mem :: "int list \<Rightarrow> (int \<Rightarrow> int) \<Rightarrow> int \<Rightarrow> int" where
   "stack_to_mem [] \<mu> k = (if k = 0 then 0 else \<mu> k)"
@@ -87,13 +87,17 @@ primrec stack_to_mem :: "int list \<Rightarrow> (int \<Rightarrow> int) \<Righta
     else stack_to_mem is \<mu> k)"
 
 fun state_convert :: "stack_state \<Rightarrow> b_assembly_state set" where
-  "state_convert (\<sigma>, \<pi>, \<omega>) = 
-    {(stack_to_mem \<sigma> \<mu>, Some 0, d, concat (map instruction_conv \<pi>), \<omega>) | d \<mu>. True }"
+  "state_convert (\<sigma>, \<pi>, s, \<omega>) = 
+    {(stack_to_mem \<sigma> \<mu>, Some 0, d, concat (map instruction_conv \<pi>), s, \<omega>) | d \<mu>. True }"
 
 (* conversion correctness *)
 
 lemma [simp]: "dom (program_convert \<Pi>) = dom \<Pi>"
   by (auto simp add: program_convert_def)
+
+lemma [simp]: "\<Pi> s = Some (\<pi>, s') \<Longrightarrow> 
+    program_convert \<Pi> s = Some (concat (map instruction_conv \<pi>), s')"
+  by (simp add: program_convert_def)
 
 lemma [simp]: "stack_to_mem \<sigma> \<mu> 0 = int (length \<sigma>)"
   by (induction \<sigma>) simp_all
@@ -141,53 +145,45 @@ lemma [simp]: "\<Sigma>\<^sub>B \<in> state_convert \<Sigma>\<^sub>S \<Longright
 lemma eval_stack_conv [simp]: "eval_stack \<Pi> \<Sigma>\<^sub>S = Some \<Sigma>\<^sub>S' \<Longrightarrow> \<Sigma>\<^sub>A \<in> state_convert \<Sigma>\<^sub>S \<Longrightarrow> 
     \<exists>\<Sigma>\<^sub>A'. \<Sigma>\<^sub>A' \<in> state_convert \<Sigma>\<^sub>S' \<and> iterate (eval_b_assembly (program_convert \<Pi>)) \<Sigma>\<^sub>A \<Sigma>\<^sub>A'"
   proof (induction \<Pi> \<Sigma>\<^sub>S rule: eval_stack.induct)
-  case (1 \<Pi> i1 i2 \<sigma> \<pi> \<omega>)
-    let ?\<pi>' = "concat (map instruction_conv \<pi>)"
-    from 1 obtain d \<mu> where M: "\<Sigma>\<^sub>A = (stack_to_mem (i1 # i2 # \<sigma>) \<mu>, Some 0, d, 
-      [CBAssm {A} (Reg M), CBAssm {D} (Reg M), ABAssm 0, 
-       CBAssm {A, M} (Decr M), CBAssm {M} DPlusM, ABAssm 0] @ ?\<pi>', \<omega>)" by fastforce
-    from 1 have S: "\<Sigma>\<^sub>S' = ((i1 + i2) # \<sigma>, \<pi>, \<omega>)" by auto
-    let ?\<mu> = "stack_to_mem (i1 # i2 # \<sigma>) \<mu>"
-    let ?\<Sigma>\<^sub>A\<^sub>1 = "(?\<mu>, Some (?\<mu> 0), d, 
-      [CBAssm {D} (Reg M), ABAssm 0, CBAssm {A, M} (Decr M), CBAssm {M} DPlusM, ABAssm 0] @ ?\<pi>', \<omega>)"
-    let ?\<Sigma>\<^sub>A\<^sub>2 = "(?\<mu>, Some (?\<mu> 0), ?\<mu> (?\<mu> 0), 
-      [ABAssm 0, CBAssm {A, M} (Decr M), CBAssm {M} DPlusM, ABAssm 0] @ ?\<pi>', \<omega>)"
-    let ?\<Sigma>\<^sub>A\<^sub>3 = "(?\<mu>, Some 0, ?\<mu> (?\<mu> 0), 
-      [CBAssm {A, M} (Decr M), CBAssm {M} DPlusM, ABAssm 0] @ ?\<pi>', \<omega>)"
-    let ?\<Sigma>\<^sub>A\<^sub>4 = "(?\<mu>(0 := ?\<mu> 0 - 1), Some (?\<mu> 0 - 1), ?\<mu> (?\<mu> 0), 
-      [CBAssm {M} DPlusM, ABAssm 0] @ ?\<pi>', \<omega>)"
-    let ?\<Sigma>\<^sub>A\<^sub>5 = "(stack_to_mem ((i1 + i2) # \<sigma>) ?\<mu>, Some (?\<mu> 0 - 1), ?\<mu> (?\<mu> 0), [ABAssm 0] @ ?\<pi>', \<omega>)"
-    let ?\<Sigma>\<^sub>A\<^sub>6 = "(stack_to_mem ((i1 + i2) # \<sigma>) ?\<mu>, Some 0, ?\<mu> (?\<mu> 0), ?\<pi>', \<omega>)"
-    from M have step1: "eval_b_assembly (program_convert \<Pi>) \<Sigma>\<^sub>A = Some ?\<Sigma>\<^sub>A\<^sub>1" by simp
-    have step2: "eval_b_assembly (program_convert \<Pi>) ?\<Sigma>\<^sub>A\<^sub>1 = Some ?\<Sigma>\<^sub>A\<^sub>2" by simp
-    have step3: "eval_b_assembly (program_convert \<Pi>) ?\<Sigma>\<^sub>A\<^sub>2 = Some ?\<Sigma>\<^sub>A\<^sub>3" by simp
-    have step4: "eval_b_assembly (program_convert \<Pi>) ?\<Sigma>\<^sub>A\<^sub>3 = Some ?\<Sigma>\<^sub>A\<^sub>4" by (simp add: Let_def)
-    have step5: "eval_b_assembly (program_convert \<Pi>) ?\<Sigma>\<^sub>A\<^sub>4 = Some ?\<Sigma>\<^sub>A\<^sub>5" by simp
-    have step6: "eval_b_assembly (program_convert \<Pi>) ?\<Sigma>\<^sub>A\<^sub>5 = Some ?\<Sigma>\<^sub>A\<^sub>6" by simp
-    from iter_two iter_prestep step1 step2 step3 have
-      "iterate (eval_b_assembly (program_convert \<Pi>)) \<Sigma>\<^sub>A ?\<Sigma>\<^sub>A\<^sub>3" by fast
-    moreover from iter_two iter_prestep step4 step5 step6 have
-      "iterate (eval_b_assembly (program_convert \<Pi>)) ?\<Sigma>\<^sub>A\<^sub>3 ?\<Sigma>\<^sub>A\<^sub>6" by fast
-    ultimately have X: "iterate (eval_b_assembly (program_convert \<Pi>)) \<Sigma>\<^sub>A ?\<Sigma>\<^sub>A\<^sub>6" by fast
-    have "?\<Sigma>\<^sub>A\<^sub>6 \<in> state_convert ((i1 + i2) # \<sigma>, \<pi>, \<omega>)" by auto
-    with X S M show ?case by metis
-  next case (2 \<Pi> i1 i2 \<sigma> \<pi> \<omega>)
+  case (1 \<Pi> \<sigma> s \<omega>)
+    then obtain d \<mu> where M: "\<Sigma>\<^sub>A = (stack_to_mem \<sigma> \<mu>, Some 0, d, [], s, \<omega>)" by fastforce
+    thus ?case
+      proof (cases "\<Pi> s")
+      case (Some \<pi>)
+        thus ?thesis
+          proof (cases \<pi>)
+          case (Pair \<pi> s')
+            with 1 Some have S: "\<Sigma>\<^sub>S' = (\<sigma>, \<pi>, s', \<omega>)" by simp
+            let ?\<pi>' = "concat (map instruction_conv \<pi>)"
+            have X: "(stack_to_mem \<sigma> \<mu>, Some 0, d, ?\<pi>', s', \<omega>) \<in> state_convert (\<sigma>, \<pi>, s', \<omega>)" 
+              by auto
+            from Some Pair have 
+              "eval_b_assembly (program_convert \<Pi>) (stack_to_mem \<sigma> \<mu>, Some 0, d, [], s, \<omega>) = 
+                Some (stack_to_mem \<sigma> \<mu>, Some 0, d, ?\<pi>', s', \<omega>)" by simp
+            with X M S iter_one show ?thesis by metis
+          qed
+      next case None
+        with 1 show ?thesis by simp
+      qed
+  next case (2 \<Pi> i1 i2 \<sigma> \<pi> s \<omega>)
     let ?\<pi>' = "concat (map instruction_conv \<pi>)"
     from 2 obtain d \<mu> where M: "\<Sigma>\<^sub>A = (stack_to_mem (i1 # i2 # \<sigma>) \<mu>, Some 0, d, 
       [CBAssm {A} (Reg M), CBAssm {D} (Reg M), ABAssm 0, 
-       CBAssm {A, M} (Decr M), CBAssm {M} MMinusD, ABAssm 0] @ ?\<pi>', \<omega>)" by fastforce
-    from 2 have S: "\<Sigma>\<^sub>S' = ((i2 - i1) # \<sigma>, \<pi>, \<omega>)" by simp
+       CBAssm {A, M} (Decr M), CBAssm {M} DPlusM, ABAssm 0] @ ?\<pi>', s, \<omega>)" by fastforce
+    from 2 have S: "\<Sigma>\<^sub>S' = ((i1 + i2) # \<sigma>, \<pi>, s, \<omega>)" by auto
     let ?\<mu> = "stack_to_mem (i1 # i2 # \<sigma>) \<mu>"
     let ?\<Sigma>\<^sub>A\<^sub>1 = "(?\<mu>, Some (?\<mu> 0), d, 
-      [CBAssm {D} (Reg M), ABAssm 0, CBAssm {A, M} (Decr M), CBAssm {M} MMinusD, ABAssm 0] @ ?\<pi>', \<omega>)"
+      [CBAssm {D} (Reg M), ABAssm 0, CBAssm {A, M} (Decr M), 
+       CBAssm {M} DPlusM, ABAssm 0] @ ?\<pi>', s, \<omega>)"
     let ?\<Sigma>\<^sub>A\<^sub>2 = "(?\<mu>, Some (?\<mu> 0), ?\<mu> (?\<mu> 0), 
-      [ABAssm 0, CBAssm {A, M} (Decr M), CBAssm {M} MMinusD, ABAssm 0] @ ?\<pi>', \<omega>)"
+      [ABAssm 0, CBAssm {A, M} (Decr M), CBAssm {M} DPlusM, ABAssm 0] @ ?\<pi>', s, \<omega>)"
     let ?\<Sigma>\<^sub>A\<^sub>3 = "(?\<mu>, Some 0, ?\<mu> (?\<mu> 0), 
-      [CBAssm {A, M} (Decr M), CBAssm {M} MMinusD, ABAssm 0] @ ?\<pi>', \<omega>)"
-    let ?\<Sigma>\<^sub>A\<^sub>4 = "(?\<mu>(0 := ?\<mu> 0 - 1), Some (?\<mu> 0 - 1), ?\<mu> (?\<mu> 0),
-      [CBAssm {M} MMinusD, ABAssm 0] @ ?\<pi>', \<omega>)"
-    let ?\<Sigma>\<^sub>A\<^sub>5 = "(stack_to_mem ((i2 - i1) # \<sigma>) ?\<mu>, Some (?\<mu> 0 - 1), ?\<mu> (?\<mu> 0), [ABAssm 0] @ ?\<pi>', \<omega>)"
-    let ?\<Sigma>\<^sub>A\<^sub>6 = "(stack_to_mem ((i2 - i1) # \<sigma>) ?\<mu>, Some 0, ?\<mu> (?\<mu> 0), ?\<pi>', \<omega>)"
+      [CBAssm {A, M} (Decr M), CBAssm {M} DPlusM, ABAssm 0] @ ?\<pi>', s, \<omega>)"
+    let ?\<Sigma>\<^sub>A\<^sub>4 = "(?\<mu>(0 := ?\<mu> 0 - 1), Some (?\<mu> 0 - 1), ?\<mu> (?\<mu> 0), 
+      [CBAssm {M} DPlusM, ABAssm 0] @ ?\<pi>', s, \<omega>)"
+    let ?\<Sigma>\<^sub>A\<^sub>5 = "(stack_to_mem ((i1 + i2) # \<sigma>) ?\<mu>, Some (?\<mu> 0 - 1), ?\<mu> (?\<mu> 0), 
+      [ABAssm 0] @ ?\<pi>', s, \<omega>)"
+    let ?\<Sigma>\<^sub>A\<^sub>6 = "(stack_to_mem ((i1 + i2) # \<sigma>) ?\<mu>, Some 0, ?\<mu> (?\<mu> 0), ?\<pi>', s, \<omega>)"
     from M have step1: "eval_b_assembly (program_convert \<Pi>) \<Sigma>\<^sub>A = Some ?\<Sigma>\<^sub>A\<^sub>1" by simp
     have step2: "eval_b_assembly (program_convert \<Pi>) ?\<Sigma>\<^sub>A\<^sub>1 = Some ?\<Sigma>\<^sub>A\<^sub>2" by simp
     have step3: "eval_b_assembly (program_convert \<Pi>) ?\<Sigma>\<^sub>A\<^sub>2 = Some ?\<Sigma>\<^sub>A\<^sub>3" by simp
@@ -199,54 +195,86 @@ lemma eval_stack_conv [simp]: "eval_stack \<Pi> \<Sigma>\<^sub>S = Some \<Sigma>
     moreover from iter_two iter_prestep step4 step5 step6 have
       "iterate (eval_b_assembly (program_convert \<Pi>)) ?\<Sigma>\<^sub>A\<^sub>3 ?\<Sigma>\<^sub>A\<^sub>6" by fast
     ultimately have X: "iterate (eval_b_assembly (program_convert \<Pi>)) \<Sigma>\<^sub>A ?\<Sigma>\<^sub>A\<^sub>6" by fast
-    have "?\<Sigma>\<^sub>A\<^sub>6 \<in> state_convert ((i2 - i1) # \<sigma>, \<pi>, \<omega>)" by auto
+    have "?\<Sigma>\<^sub>A\<^sub>6 \<in> state_convert ((i1 + i2) # \<sigma>, \<pi>, s, \<omega>)" by auto
     with X S M show ?case by metis
-  next case (3 \<Pi> i1 \<sigma> \<pi> \<omega>)
+  next case (3 \<Pi> i1 i2 \<sigma> \<pi> s \<omega>)
     let ?\<pi>' = "concat (map instruction_conv \<pi>)"
-    from 3 obtain d \<mu> where M: "\<Sigma>\<^sub>A = (stack_to_mem (i1 # \<sigma>) \<mu>, Some 0, d, 
-      [CBAssm {A} (Reg M), CBAssm {M} (NegR M), ABAssm 0] @ ?\<pi>', \<omega>)" by fastforce
-    from 3 have S: "\<Sigma>\<^sub>S' = (-i1 # \<sigma>, \<pi>, \<omega>)" by simp
+    from 3 obtain d \<mu> where M: "\<Sigma>\<^sub>A = (stack_to_mem (i1 # i2 # \<sigma>) \<mu>, Some 0, d, 
+      [CBAssm {A} (Reg M), CBAssm {D} (Reg M), ABAssm 0, 
+       CBAssm {A, M} (Decr M), CBAssm {M} MMinusD, ABAssm 0] @ ?\<pi>', s, \<omega>)" by fastforce
+    from 3 have S: "\<Sigma>\<^sub>S' = ((i2 - i1) # \<sigma>, \<pi>, s, \<omega>)" by simp
+    let ?\<mu> = "stack_to_mem (i1 # i2 # \<sigma>) \<mu>"
+    let ?\<Sigma>\<^sub>A\<^sub>1 = "(?\<mu>, Some (?\<mu> 0), d, 
+      [CBAssm {D} (Reg M), ABAssm 0, 
+       CBAssm {A, M} (Decr M), CBAssm {M} MMinusD, ABAssm 0] @ ?\<pi>', s, \<omega>)"
+    let ?\<Sigma>\<^sub>A\<^sub>2 = "(?\<mu>, Some (?\<mu> 0), ?\<mu> (?\<mu> 0), 
+      [ABAssm 0, CBAssm {A, M} (Decr M), CBAssm {M} MMinusD, ABAssm 0] @ ?\<pi>', s, \<omega>)"
+    let ?\<Sigma>\<^sub>A\<^sub>3 = "(?\<mu>, Some 0, ?\<mu> (?\<mu> 0), 
+      [CBAssm {A, M} (Decr M), CBAssm {M} MMinusD, ABAssm 0] @ ?\<pi>', s, \<omega>)"
+    let ?\<Sigma>\<^sub>A\<^sub>4 = "(?\<mu>(0 := ?\<mu> 0 - 1), Some (?\<mu> 0 - 1), ?\<mu> (?\<mu> 0),
+      [CBAssm {M} MMinusD, ABAssm 0] @ ?\<pi>', s, \<omega>)"
+    let ?\<Sigma>\<^sub>A\<^sub>5 = "(stack_to_mem ((i2 - i1) # \<sigma>) ?\<mu>, Some (?\<mu> 0 - 1), ?\<mu> (?\<mu> 0), 
+      [ABAssm 0] @ ?\<pi>', s, \<omega>)"
+    let ?\<Sigma>\<^sub>A\<^sub>6 = "(stack_to_mem ((i2 - i1) # \<sigma>) ?\<mu>, Some 0, ?\<mu> (?\<mu> 0), ?\<pi>', s, \<omega>)"
+    from M have step1: "eval_b_assembly (program_convert \<Pi>) \<Sigma>\<^sub>A = Some ?\<Sigma>\<^sub>A\<^sub>1" by simp
+    have step2: "eval_b_assembly (program_convert \<Pi>) ?\<Sigma>\<^sub>A\<^sub>1 = Some ?\<Sigma>\<^sub>A\<^sub>2" by simp
+    have step3: "eval_b_assembly (program_convert \<Pi>) ?\<Sigma>\<^sub>A\<^sub>2 = Some ?\<Sigma>\<^sub>A\<^sub>3" by simp
+    have step4: "eval_b_assembly (program_convert \<Pi>) ?\<Sigma>\<^sub>A\<^sub>3 = Some ?\<Sigma>\<^sub>A\<^sub>4" by (simp add: Let_def)
+    have step5: "eval_b_assembly (program_convert \<Pi>) ?\<Sigma>\<^sub>A\<^sub>4 = Some ?\<Sigma>\<^sub>A\<^sub>5" by simp
+    have step6: "eval_b_assembly (program_convert \<Pi>) ?\<Sigma>\<^sub>A\<^sub>5 = Some ?\<Sigma>\<^sub>A\<^sub>6" by simp
+    from iter_two iter_prestep step1 step2 step3 have
+      "iterate (eval_b_assembly (program_convert \<Pi>)) \<Sigma>\<^sub>A ?\<Sigma>\<^sub>A\<^sub>3" by fast
+    moreover from iter_two iter_prestep step4 step5 step6 have
+      "iterate (eval_b_assembly (program_convert \<Pi>)) ?\<Sigma>\<^sub>A\<^sub>3 ?\<Sigma>\<^sub>A\<^sub>6" by fast
+    ultimately have X: "iterate (eval_b_assembly (program_convert \<Pi>)) \<Sigma>\<^sub>A ?\<Sigma>\<^sub>A\<^sub>6" by fast
+    have "?\<Sigma>\<^sub>A\<^sub>6 \<in> state_convert ((i2 - i1) # \<sigma>, \<pi>, s, \<omega>)" by auto
+    with X S M show ?case by metis
+  next case (4 \<Pi> i1 \<sigma> \<pi> s \<omega>)
+    let ?\<pi>' = "concat (map instruction_conv \<pi>)"
+    from 4 obtain d \<mu> where M: "\<Sigma>\<^sub>A = (stack_to_mem (i1 # \<sigma>) \<mu>, Some 0, d, 
+      [CBAssm {A} (Reg M), CBAssm {M} (NegR M), ABAssm 0] @ ?\<pi>', s, \<omega>)" by fastforce
+    from 4 have S: "\<Sigma>\<^sub>S' = (-i1 # \<sigma>, \<pi>, s, \<omega>)" by simp
     let ?\<mu> = "stack_to_mem (i1 # \<sigma>) \<mu>"
-    let ?\<Sigma>\<^sub>A\<^sub>1 = "(?\<mu>, Some (?\<mu> 0), d, [CBAssm {M} (NegR M), ABAssm 0] @ ?\<pi>', \<omega>)"
-    let ?\<Sigma>\<^sub>A\<^sub>2 = "(?\<mu>(?\<mu> 0 := - ?\<mu> (?\<mu> 0)), Some (?\<mu> 0), d, [ABAssm 0] @ ?\<pi>', \<omega>)"
-    let ?\<Sigma>\<^sub>A\<^sub>3 = "(?\<mu>(?\<mu> 0 := - ?\<mu> (?\<mu> 0)), Some 0, d, ?\<pi>', \<omega>)"
+    let ?\<Sigma>\<^sub>A\<^sub>1 = "(?\<mu>, Some (?\<mu> 0), d, [CBAssm {M} (NegR M), ABAssm 0] @ ?\<pi>', s, \<omega>)"
+    let ?\<Sigma>\<^sub>A\<^sub>2 = "(?\<mu>(?\<mu> 0 := - ?\<mu> (?\<mu> 0)), Some (?\<mu> 0), d, [ABAssm 0] @ ?\<pi>', s, \<omega>)"
+    let ?\<Sigma>\<^sub>A\<^sub>3 = "(?\<mu>(?\<mu> 0 := - ?\<mu> (?\<mu> 0)), Some 0, d, ?\<pi>', s, \<omega>)"
     from M have step1: "eval_b_assembly (program_convert \<Pi>) \<Sigma>\<^sub>A = Some ?\<Sigma>\<^sub>A\<^sub>1" by simp
     have step2: "eval_b_assembly (program_convert \<Pi>) ?\<Sigma>\<^sub>A\<^sub>1 = Some ?\<Sigma>\<^sub>A\<^sub>2" by simp
     have "eval_b_assembly (program_convert \<Pi>) ?\<Sigma>\<^sub>A\<^sub>2 = Some ?\<Sigma>\<^sub>A\<^sub>3" by simp
     with iter_two iter_prestep step1 step2 have X:
       "iterate (eval_b_assembly (program_convert \<Pi>)) \<Sigma>\<^sub>A ?\<Sigma>\<^sub>A\<^sub>3" by fast
     have "(stack_to_mem (i1 # \<sigma>) \<mu>)(1 + int (length \<sigma>) := - i1) = stack_to_mem (- i1 # \<sigma>) \<mu>" by auto
-    hence "?\<Sigma>\<^sub>A\<^sub>3 \<in> state_convert ((-i1) # \<sigma>, \<pi>, \<omega>)" by auto
+    hence "?\<Sigma>\<^sub>A\<^sub>3 \<in> state_convert ((-i1) # \<sigma>, \<pi>, s, \<omega>)" by auto
     with X S M show ?case by metis
-  next case (4 \<Pi> i1 i2 \<sigma> \<pi> \<omega>)
+  next case (5 \<Pi> i1 i2 \<sigma> \<pi> s \<omega>)
     let ?\<pi>' = "concat (map instruction_conv \<pi>)"
-    from 4 obtain d \<mu> where M: "\<Sigma>\<^sub>A = (stack_to_mem (i1 # i2 # \<sigma>) \<mu>, Some 0, d, 
+    from 5 obtain d \<mu> where M: "\<Sigma>\<^sub>A = (stack_to_mem (i1 # i2 # \<sigma>) \<mu>, Some 0, d, 
       [CBAssm {A} (Reg M), CBAssm {D} (Reg M), ABAssm 0, 
        CBAssm {A, M} (Decr M), CBAssm {D} MMinusD, 
-       IBAssm {EQ} [CBAssm {M} One] [CBAssm {M} Zero], ABAssm 0] @ ?\<pi>', \<omega>)" by fastforce
-    from 4 have S: "\<Sigma>\<^sub>S' = (unboolify (i2 = i1) # \<sigma>, \<pi>, \<omega>)" by simp
+       IBAssm {EQ} [CBAssm {M} One] [CBAssm {M} Zero], ABAssm 0] @ ?\<pi>', s, \<omega>)" by fastforce
+    from 5 have S: "\<Sigma>\<^sub>S' = (unboolify (i2 = i1) # \<sigma>, \<pi>, s, \<omega>)" by simp
     let ?\<mu> = "stack_to_mem (i1 # i2 # \<sigma>) \<mu>"
     let ?\<Sigma>\<^sub>A\<^sub>1 = "(?\<mu>, Some (?\<mu> 0), d, 
       [CBAssm {D} (Reg M), ABAssm 0, CBAssm {A, M} (Decr M), CBAssm {D} MMinusD, 
-       IBAssm {EQ} [CBAssm {M} One] [CBAssm {M} Zero], ABAssm 0] @ ?\<pi>', \<omega>)"
+       IBAssm {EQ} [CBAssm {M} One] [CBAssm {M} Zero], ABAssm 0] @ ?\<pi>', s, \<omega>)"
     let ?\<Sigma>\<^sub>A\<^sub>2 = "(?\<mu>, Some (?\<mu> 0), ?\<mu> (?\<mu> 0), 
       [ABAssm 0, CBAssm {A, M} (Decr M), CBAssm {D} MMinusD, 
-       IBAssm {EQ} [CBAssm {M} One] [CBAssm {M} Zero], ABAssm 0] @ ?\<pi>', \<omega>)"
+       IBAssm {EQ} [CBAssm {M} One] [CBAssm {M} Zero], ABAssm 0] @ ?\<pi>', s, \<omega>)"
     let ?\<Sigma>\<^sub>A\<^sub>3 = "(?\<mu>, Some 0, ?\<mu> (?\<mu> 0), 
       [CBAssm {A, M} (Decr M), CBAssm {D} MMinusD, 
-       IBAssm {EQ} [CBAssm {M} One] [CBAssm {M} Zero], ABAssm 0] @ ?\<pi>', \<omega>)"
+       IBAssm {EQ} [CBAssm {M} One] [CBAssm {M} Zero], ABAssm 0] @ ?\<pi>', s, \<omega>)"
     let ?\<Sigma>\<^sub>A\<^sub>4 = "(?\<mu>(0 := ?\<mu> 0 - 1), Some (?\<mu> 0 - 1), ?\<mu> (?\<mu> 0), 
-      [CBAssm {D} MMinusD, IBAssm {EQ} [CBAssm {M} One] [CBAssm {M} Zero], ABAssm 0] @ ?\<pi>', \<omega>)"
+      [CBAssm {D} MMinusD, IBAssm {EQ} [CBAssm {M} One] [CBAssm {M} Zero], ABAssm 0] @ ?\<pi>', s, \<omega>)"
     let ?\<Sigma>\<^sub>A\<^sub>5 = "(?\<mu>(0 := ?\<mu> 0 - 1), Some (?\<mu> 0 - 1), ?\<mu> (?\<mu> 0 - 1) - ?\<mu> (?\<mu> 0), 
-      [IBAssm {EQ} [CBAssm {M} One] [CBAssm {M} Zero], ABAssm 0] @ ?\<pi>', \<omega>)"
+      [IBAssm {EQ} [CBAssm {M} One] [CBAssm {M} Zero], ABAssm 0] @ ?\<pi>', s, \<omega>)"
     let ?\<Sigma>\<^sub>A\<^sub>6\<^sub>t = "(?\<mu>(0 := ?\<mu> 0 - 1), Some (?\<mu> 0 - 1), ?\<mu> (?\<mu> 0 - 1) - ?\<mu> (?\<mu> 0), 
-      [CBAssm {M} One, ABAssm 0] @ ?\<pi>', \<omega>)"
+      [CBAssm {M} One, ABAssm 0] @ ?\<pi>', s, \<omega>)"
     let ?\<Sigma>\<^sub>A\<^sub>6\<^sub>f = "(?\<mu>(0 := ?\<mu> 0 - 1), Some (?\<mu> 0 - 1), ?\<mu> (?\<mu> 0 - 1) - ?\<mu> (?\<mu> 0), 
-      [CBAssm {M} Zero, ABAssm 0] @ ?\<pi>', \<omega>)"
+      [CBAssm {M} Zero, ABAssm 0] @ ?\<pi>', s, \<omega>)"
     let ?\<Sigma>\<^sub>A\<^sub>7 = "(stack_to_mem (unboolify (i2 = i1) # \<sigma>) ?\<mu>, Some (?\<mu> 0 - 1), 
-      ?\<mu> (?\<mu> 0 - 1) - ?\<mu> (?\<mu> 0), [ABAssm 0] @ ?\<pi>', \<omega>)"
+      ?\<mu> (?\<mu> 0 - 1) - ?\<mu> (?\<mu> 0), [ABAssm 0] @ ?\<pi>', s, \<omega>)"
     let ?\<Sigma>\<^sub>A\<^sub>8 = "(stack_to_mem (unboolify (i2 = i1) # \<sigma>) ?\<mu>, Some 0, 
-      ?\<mu> (?\<mu> 0 - 1) - ?\<mu> (?\<mu> 0), ?\<pi>', \<omega>)"
+      ?\<mu> (?\<mu> 0 - 1) - ?\<mu> (?\<mu> 0), ?\<pi>', s, \<omega>)"
     from M have step1: "eval_b_assembly (program_convert \<Pi>) \<Sigma>\<^sub>A = Some ?\<Sigma>\<^sub>A\<^sub>1" by simp
     have step2: "eval_b_assembly (program_convert \<Pi>) ?\<Sigma>\<^sub>A\<^sub>1 = Some ?\<Sigma>\<^sub>A\<^sub>2" by simp
     have step3: "eval_b_assembly (program_convert \<Pi>) ?\<Sigma>\<^sub>A\<^sub>2 = Some ?\<Sigma>\<^sub>A\<^sub>3" by simp
@@ -273,37 +301,37 @@ lemma eval_stack_conv [simp]: "eval_stack \<Pi> \<Sigma>\<^sub>S = Some \<Sigma>
         with iter_two iter_prestep step6f step7f step8 show ?thesis by fast
       qed
     with Y iter_many have X: "iterate (eval_b_assembly (program_convert \<Pi>)) \<Sigma>\<^sub>A ?\<Sigma>\<^sub>A\<^sub>8" by fast
-    have "?\<Sigma>\<^sub>A\<^sub>8 \<in> state_convert (unboolify (i2 = i1) # \<sigma>, \<pi>, \<omega>)" by fastforce
+    have "?\<Sigma>\<^sub>A\<^sub>8 \<in> state_convert (unboolify (i2 = i1) # \<sigma>, \<pi>, s, \<omega>)" by fastforce
     with X S show ?case by metis
-  next case (5 \<Pi> i1 i2 \<sigma> \<pi> \<omega>)
+  next case (6 \<Pi> i1 i2 \<sigma> \<pi> s \<omega>)
     let ?\<pi>' = "concat (map instruction_conv \<pi>)"
-    from 5 obtain d \<mu> where M: "\<Sigma>\<^sub>A = (stack_to_mem (i1 # i2 # \<sigma>) \<mu>, Some 0, d, 
+    from 6 obtain d \<mu> where M: "\<Sigma>\<^sub>A = (stack_to_mem (i1 # i2 # \<sigma>) \<mu>, Some 0, d, 
       [CBAssm {A} (Reg M), CBAssm {D} (Reg M), ABAssm 0, 
        CBAssm {A, M} (Decr M), CBAssm {D} MMinusD, 
-       IBAssm {GT} [CBAssm {M} One] [CBAssm {M} Zero], ABAssm 0] @ ?\<pi>', \<omega>)" by fastforce
-    from 5 have S: "\<Sigma>\<^sub>S' = (unboolify (i2 > i1) # \<sigma>, \<pi>, \<omega>)" by simp
+       IBAssm {GT} [CBAssm {M} One] [CBAssm {M} Zero], ABAssm 0] @ ?\<pi>', s, \<omega>)" by fastforce
+    from 6 have S: "\<Sigma>\<^sub>S' = (unboolify (i2 > i1) # \<sigma>, \<pi>, s, \<omega>)" by simp
     let ?\<mu> = "stack_to_mem (i1 # i2 # \<sigma>) \<mu>"
     let ?\<Sigma>\<^sub>A\<^sub>1 = "(?\<mu>, Some (?\<mu> 0), d, 
       [CBAssm {D} (Reg M), ABAssm 0, CBAssm {A, M} (Decr M), CBAssm {D} MMinusD, 
-       IBAssm {GT} [CBAssm {M} One] [CBAssm {M} Zero], ABAssm 0] @ ?\<pi>', \<omega>)"
+       IBAssm {GT} [CBAssm {M} One] [CBAssm {M} Zero], ABAssm 0] @ ?\<pi>', s, \<omega>)"
     let ?\<Sigma>\<^sub>A\<^sub>2 = "(?\<mu>, Some (?\<mu> 0), ?\<mu> (?\<mu> 0), 
       [ABAssm 0, CBAssm {A, M} (Decr M), CBAssm {D} MMinusD, 
-       IBAssm {GT} [CBAssm {M} One] [CBAssm {M} Zero], ABAssm 0] @ ?\<pi>', \<omega>)"
+       IBAssm {GT} [CBAssm {M} One] [CBAssm {M} Zero], ABAssm 0] @ ?\<pi>', s, \<omega>)"
     let ?\<Sigma>\<^sub>A\<^sub>3 = "(?\<mu>, Some 0, ?\<mu> (?\<mu> 0), 
       [CBAssm {A, M} (Decr M), CBAssm {D} MMinusD, 
-       IBAssm {GT} [CBAssm {M} One] [CBAssm {M} Zero], ABAssm 0] @ ?\<pi>', \<omega>)"
+       IBAssm {GT} [CBAssm {M} One] [CBAssm {M} Zero], ABAssm 0] @ ?\<pi>', s, \<omega>)"
     let ?\<Sigma>\<^sub>A\<^sub>4 = "(?\<mu>(0 := ?\<mu> 0 - 1), Some (?\<mu> 0 - 1), ?\<mu> (?\<mu> 0), 
-      [CBAssm {D} MMinusD, IBAssm {GT} [CBAssm {M} One] [CBAssm {M} Zero], ABAssm 0] @ ?\<pi>', \<omega>)"
+      [CBAssm {D} MMinusD, IBAssm {GT} [CBAssm {M} One] [CBAssm {M} Zero], ABAssm 0] @ ?\<pi>', s, \<omega>)"
     let ?\<Sigma>\<^sub>A\<^sub>5 = "(?\<mu>(0 := ?\<mu> 0 - 1), Some (?\<mu> 0 - 1), ?\<mu> (?\<mu> 0 - 1) - ?\<mu> (?\<mu> 0), 
-      [IBAssm {GT} [CBAssm {M} One] [CBAssm {M} Zero], ABAssm 0] @ ?\<pi>', \<omega>)"
+      [IBAssm {GT} [CBAssm {M} One] [CBAssm {M} Zero], ABAssm 0] @ ?\<pi>', s, \<omega>)"
     let ?\<Sigma>\<^sub>A\<^sub>6\<^sub>t = "(?\<mu>(0 := ?\<mu> 0 - 1), Some (?\<mu> 0 - 1), ?\<mu> (?\<mu> 0 - 1) - ?\<mu> (?\<mu> 0), 
-      [CBAssm {M} One, ABAssm 0] @ ?\<pi>', \<omega>)"
+      [CBAssm {M} One, ABAssm 0] @ ?\<pi>', s, \<omega>)"
     let ?\<Sigma>\<^sub>A\<^sub>6\<^sub>f = "(?\<mu>(0 := ?\<mu> 0 - 1), Some (?\<mu> 0 - 1), ?\<mu> (?\<mu> 0 - 1) - ?\<mu> (?\<mu> 0), 
-      [CBAssm {M} Zero, ABAssm 0] @ ?\<pi>', \<omega>)"
+      [CBAssm {M} Zero, ABAssm 0] @ ?\<pi>', s, \<omega>)"
     let ?\<Sigma>\<^sub>A\<^sub>7 = "(stack_to_mem (unboolify (i2 > i1) # \<sigma>) ?\<mu>, Some (?\<mu> 0 - 1), 
-      ?\<mu> (?\<mu> 0 - 1) - ?\<mu> (?\<mu> 0), [ABAssm 0] @ ?\<pi>', \<omega>)"
+      ?\<mu> (?\<mu> 0 - 1) - ?\<mu> (?\<mu> 0), [ABAssm 0] @ ?\<pi>', s, \<omega>)"
     let ?\<Sigma>\<^sub>A\<^sub>8 = "(stack_to_mem (unboolify (i2 > i1) # \<sigma>) ?\<mu>, Some 0, 
-      ?\<mu> (?\<mu> 0 - 1) - ?\<mu> (?\<mu> 0), ?\<pi>', \<omega>)"
+      ?\<mu> (?\<mu> 0 - 1) - ?\<mu> (?\<mu> 0), ?\<pi>', s, \<omega>)"
     from M have step1: "eval_b_assembly (program_convert \<Pi>) \<Sigma>\<^sub>A = Some ?\<Sigma>\<^sub>A\<^sub>1" by simp
     have step2: "eval_b_assembly (program_convert \<Pi>) ?\<Sigma>\<^sub>A\<^sub>1 = Some ?\<Sigma>\<^sub>A\<^sub>2" by simp
     have step3: "eval_b_assembly (program_convert \<Pi>) ?\<Sigma>\<^sub>A\<^sub>2 = Some ?\<Sigma>\<^sub>A\<^sub>3" by simp
@@ -330,37 +358,37 @@ lemma eval_stack_conv [simp]: "eval_stack \<Pi> \<Sigma>\<^sub>S = Some \<Sigma>
         with iter_two iter_prestep step6f step7f step8 show ?thesis by fast
       qed
     with Y iter_many have X: "iterate (eval_b_assembly (program_convert \<Pi>)) \<Sigma>\<^sub>A ?\<Sigma>\<^sub>A\<^sub>8" by fast
-    have "?\<Sigma>\<^sub>A\<^sub>8 \<in> state_convert (unboolify (i2 > i1) # \<sigma>, \<pi>, \<omega>)" by fastforce
+    have "?\<Sigma>\<^sub>A\<^sub>8 \<in> state_convert (unboolify (i2 > i1) # \<sigma>, \<pi>, s, \<omega>)" by fastforce
     with X S show ?case by metis
-  next case (6 \<Pi> i1 i2 \<sigma> \<pi> \<omega>)
+  next case (7 \<Pi> i1 i2 \<sigma> \<pi> s \<omega>)
     let ?\<pi>' = "concat (map instruction_conv \<pi>)"
-    from 6 obtain d \<mu> where M: "\<Sigma>\<^sub>A = (stack_to_mem (i1 # i2 # \<sigma>) \<mu>, Some 0, d, 
+    from 7 obtain d \<mu> where M: "\<Sigma>\<^sub>A = (stack_to_mem (i1 # i2 # \<sigma>) \<mu>, Some 0, d, 
       [CBAssm {A} (Reg M), CBAssm {D} (Reg M), ABAssm 0, 
        CBAssm {A, M} (Decr M), CBAssm {D} MMinusD, 
-       IBAssm {LT} [CBAssm {M} One] [CBAssm {M} Zero], ABAssm 0] @ ?\<pi>', \<omega>)" by fastforce
-    from 6 have S: "\<Sigma>\<^sub>S' = (unboolify (i2 < i1) # \<sigma>, \<pi>, \<omega>)" by simp
+       IBAssm {LT} [CBAssm {M} One] [CBAssm {M} Zero], ABAssm 0] @ ?\<pi>', s, \<omega>)" by fastforce
+    from 7 have S: "\<Sigma>\<^sub>S' = (unboolify (i2 < i1) # \<sigma>, \<pi>, s, \<omega>)" by simp
     let ?\<mu> = "stack_to_mem (i1 # i2 # \<sigma>) \<mu>"
     let ?\<Sigma>\<^sub>A\<^sub>1 = "(?\<mu>, Some (?\<mu> 0), d, 
       [CBAssm {D} (Reg M), ABAssm 0, CBAssm {A, M} (Decr M), CBAssm {D} MMinusD, 
-       IBAssm {LT} [CBAssm {M} One] [CBAssm {M} Zero], ABAssm 0] @ ?\<pi>', \<omega>)"
+       IBAssm {LT} [CBAssm {M} One] [CBAssm {M} Zero], ABAssm 0] @ ?\<pi>', s, \<omega>)"
     let ?\<Sigma>\<^sub>A\<^sub>2 = "(?\<mu>, Some (?\<mu> 0), ?\<mu> (?\<mu> 0), 
       [ABAssm 0, CBAssm {A, M} (Decr M), CBAssm {D} MMinusD, 
-       IBAssm {LT} [CBAssm {M} One] [CBAssm {M} Zero], ABAssm 0] @ ?\<pi>', \<omega>)"
+       IBAssm {LT} [CBAssm {M} One] [CBAssm {M} Zero], ABAssm 0] @ ?\<pi>', s, \<omega>)"
     let ?\<Sigma>\<^sub>A\<^sub>3 = "(?\<mu>, Some 0, ?\<mu> (?\<mu> 0), 
       [CBAssm {A, M} (Decr M), CBAssm {D} MMinusD, 
-       IBAssm {LT} [CBAssm {M} One] [CBAssm {M} Zero], ABAssm 0] @ ?\<pi>', \<omega>)"
+       IBAssm {LT} [CBAssm {M} One] [CBAssm {M} Zero], ABAssm 0] @ ?\<pi>', s, \<omega>)"
     let ?\<Sigma>\<^sub>A\<^sub>4 = "(?\<mu>(0 := ?\<mu> 0 - 1), Some (?\<mu> 0 - 1), ?\<mu> (?\<mu> 0), 
-      [CBAssm {D} MMinusD, IBAssm {LT} [CBAssm {M} One] [CBAssm {M} Zero], ABAssm 0] @ ?\<pi>', \<omega>)"
+      [CBAssm {D} MMinusD, IBAssm {LT} [CBAssm {M} One] [CBAssm {M} Zero], ABAssm 0] @ ?\<pi>', s, \<omega>)"
     let ?\<Sigma>\<^sub>A\<^sub>5 = "(?\<mu>(0 := ?\<mu> 0 - 1), Some (?\<mu> 0 - 1), ?\<mu> (?\<mu> 0 - 1) - ?\<mu> (?\<mu> 0), 
-      [IBAssm {LT} [CBAssm {M} One] [CBAssm {M} Zero], ABAssm 0] @ ?\<pi>', \<omega>)"
+      [IBAssm {LT} [CBAssm {M} One] [CBAssm {M} Zero], ABAssm 0] @ ?\<pi>', s, \<omega>)"
     let ?\<Sigma>\<^sub>A\<^sub>6\<^sub>t = "(?\<mu>(0 := ?\<mu> 0 - 1), Some (?\<mu> 0 - 1), ?\<mu> (?\<mu> 0 - 1) - ?\<mu> (?\<mu> 0), 
-      [CBAssm {M} One, ABAssm 0] @ ?\<pi>', \<omega>)"
+      [CBAssm {M} One, ABAssm 0] @ ?\<pi>', s, \<omega>)"
     let ?\<Sigma>\<^sub>A\<^sub>6\<^sub>f = "(?\<mu>(0 := ?\<mu> 0 - 1), Some (?\<mu> 0 - 1), ?\<mu> (?\<mu> 0 - 1) - ?\<mu> (?\<mu> 0), 
-      [CBAssm {M} Zero, ABAssm 0] @ ?\<pi>', \<omega>)"
+      [CBAssm {M} Zero, ABAssm 0] @ ?\<pi>', s, \<omega>)"
     let ?\<Sigma>\<^sub>A\<^sub>7 = "(stack_to_mem (unboolify (i2 < i1) # \<sigma>) ?\<mu>, Some (?\<mu> 0 - 1), 
-      ?\<mu> (?\<mu> 0 - 1) - ?\<mu> (?\<mu> 0), [ABAssm 0] @ ?\<pi>', \<omega>)"
+      ?\<mu> (?\<mu> 0 - 1) - ?\<mu> (?\<mu> 0), [ABAssm 0] @ ?\<pi>', s, \<omega>)"
     let ?\<Sigma>\<^sub>A\<^sub>8 = "(stack_to_mem (unboolify (i2 < i1) # \<sigma>) ?\<mu>, Some 0, 
-      ?\<mu> (?\<mu> 0 - 1) - ?\<mu> (?\<mu> 0), ?\<pi>', \<omega>)"
+      ?\<mu> (?\<mu> 0 - 1) - ?\<mu> (?\<mu> 0), ?\<pi>', s, \<omega>)"
     from M have step1: "eval_b_assembly (program_convert \<Pi>) \<Sigma>\<^sub>A = Some ?\<Sigma>\<^sub>A\<^sub>1" by simp
     have step2: "eval_b_assembly (program_convert \<Pi>) ?\<Sigma>\<^sub>A\<^sub>1 = Some ?\<Sigma>\<^sub>A\<^sub>2" by simp
     have step3: "eval_b_assembly (program_convert \<Pi>) ?\<Sigma>\<^sub>A\<^sub>2 = Some ?\<Sigma>\<^sub>A\<^sub>3" by simp
@@ -387,59 +415,27 @@ lemma eval_stack_conv [simp]: "eval_stack \<Pi> \<Sigma>\<^sub>S = Some \<Sigma>
         with iter_two iter_prestep step6f step7f step8 show ?thesis by fast
       qed
     with Y iter_many have X: "iterate (eval_b_assembly (program_convert \<Pi>)) \<Sigma>\<^sub>A ?\<Sigma>\<^sub>A\<^sub>8" by fast
-    have "?\<Sigma>\<^sub>A\<^sub>8 \<in> state_convert (unboolify (i2 < i1) # \<sigma>, \<pi>, \<omega>)" by fastforce
+    have "?\<Sigma>\<^sub>A\<^sub>8 \<in> state_convert (unboolify (i2 < i1) # \<sigma>, \<pi>, s, \<omega>)" by fastforce
     with X S show ?case by metis
-  next case (7 \<Pi> i1 i2 \<sigma> \<pi> \<omega>)
-    let ?\<pi>' = "concat (map instruction_conv \<pi>)"
-    from 7 obtain d \<mu> where M: "\<Sigma>\<^sub>A = (stack_to_mem (i1 # i2 # \<sigma>) \<mu>, Some 0, d, 
-      [CBAssm {A} (Reg M), CBAssm {D} (Reg M), ABAssm 0, 
-       CBAssm {A, M} (Decr M), CBAssm {M} DAndM, ABAssm 0] @ ?\<pi>', \<omega>)" by fastforce
-    from 7 have S: "\<Sigma>\<^sub>S' = (unboolify (boolify i1 \<and> boolify i2) # \<sigma>, \<pi>, \<omega>)" by simp
-    let ?\<mu> = "stack_to_mem (i1 # i2 # \<sigma>) \<mu>"
-    let ?\<Sigma>\<^sub>A\<^sub>1 = "(?\<mu>, Some (?\<mu> 0), d, 
-      [CBAssm {D} (Reg M), ABAssm 0, CBAssm {A, M} (Decr M), CBAssm {M} DAndM, ABAssm 0] @ ?\<pi>', \<omega>)"
-    let ?\<Sigma>\<^sub>A\<^sub>2 = "(?\<mu>, Some (?\<mu> 0), ?\<mu> (?\<mu> 0), 
-      [ABAssm 0, CBAssm {A, M} (Decr M), CBAssm {M} DAndM, ABAssm 0] @ ?\<pi>', \<omega>)"
-    let ?\<Sigma>\<^sub>A\<^sub>3 = "(?\<mu>, Some 0, ?\<mu> (?\<mu> 0), 
-      [CBAssm {A, M} (Decr M), CBAssm {M} DAndM, ABAssm 0] @ ?\<pi>', \<omega>)"
-    let ?\<Sigma>\<^sub>A\<^sub>4 = "(?\<mu>(0 := ?\<mu> 0 - 1), Some (?\<mu> 0 - 1), ?\<mu> (?\<mu> 0), 
-      [CBAssm {M} DAndM, ABAssm 0] @ ?\<pi>', \<omega>)"
-    let ?\<Sigma>\<^sub>A\<^sub>5 = "(stack_to_mem (unboolify (boolify i1 \<and> boolify i2) # \<sigma>) ?\<mu>, Some (?\<mu> 0 - 1), 
-      ?\<mu> (?\<mu> 0), [ABAssm 0] @ ?\<pi>', \<omega>)"
-    let ?\<Sigma>\<^sub>A\<^sub>6 = "(stack_to_mem (unboolify (boolify i1 \<and> boolify i2) # \<sigma>) ?\<mu>, Some 0, 
-      ?\<mu> (?\<mu> 0), ?\<pi>', \<omega>)"
-    from M have step1: "eval_b_assembly (program_convert \<Pi>) \<Sigma>\<^sub>A = Some ?\<Sigma>\<^sub>A\<^sub>1" by simp
-    have step2: "eval_b_assembly (program_convert \<Pi>) ?\<Sigma>\<^sub>A\<^sub>1 = Some ?\<Sigma>\<^sub>A\<^sub>2" by simp
-    have step3: "eval_b_assembly (program_convert \<Pi>) ?\<Sigma>\<^sub>A\<^sub>2 = Some ?\<Sigma>\<^sub>A\<^sub>3" by simp
-    have step4: "eval_b_assembly (program_convert \<Pi>) ?\<Sigma>\<^sub>A\<^sub>3 = Some ?\<Sigma>\<^sub>A\<^sub>4" by (simp add: Let_def)
-    have step5: "eval_b_assembly (program_convert \<Pi>) ?\<Sigma>\<^sub>A\<^sub>4 = Some ?\<Sigma>\<^sub>A\<^sub>5" by simp
-    have step6: "eval_b_assembly (program_convert \<Pi>) ?\<Sigma>\<^sub>A\<^sub>5 = Some ?\<Sigma>\<^sub>A\<^sub>6" by simp
-    from iter_two iter_prestep step1 step2 step3 have
-      "iterate (eval_b_assembly (program_convert \<Pi>)) \<Sigma>\<^sub>A ?\<Sigma>\<^sub>A\<^sub>3" by fast
-    moreover from iter_two iter_prestep step4 step5 step6 have
-      "iterate (eval_b_assembly (program_convert \<Pi>)) ?\<Sigma>\<^sub>A\<^sub>3 ?\<Sigma>\<^sub>A\<^sub>6" by fast
-    ultimately have X: "iterate (eval_b_assembly (program_convert \<Pi>)) \<Sigma>\<^sub>A ?\<Sigma>\<^sub>A\<^sub>6" by fast
-    have "?\<Sigma>\<^sub>A\<^sub>6 \<in> state_convert (unboolify (boolify i1 \<and> boolify i2) # \<sigma>, \<pi>, \<omega>)" by auto
-    with X S M show ?case by metis
-  next case (8 \<Pi> i1 i2 \<sigma> \<pi> \<omega>)
+  next case (8 \<Pi> i1 i2 \<sigma> \<pi> s \<omega>)
     let ?\<pi>' = "concat (map instruction_conv \<pi>)"
     from 8 obtain d \<mu> where M: "\<Sigma>\<^sub>A = (stack_to_mem (i1 # i2 # \<sigma>) \<mu>, Some 0, d, 
       [CBAssm {A} (Reg M), CBAssm {D} (Reg M), ABAssm 0, 
-       CBAssm {A, M} (Decr M), CBAssm {M} DOrM, ABAssm 0] @ ?\<pi>', \<omega>)" by fastforce
-    from 8 have S: "\<Sigma>\<^sub>S' = (unboolify (boolify i1 \<or> boolify i2) # \<sigma>, \<pi>, \<omega>)" by simp
+       CBAssm {A, M} (Decr M), CBAssm {M} DAndM, ABAssm 0] @ ?\<pi>', s, \<omega>)" by fastforce
+    from 8 have S: "\<Sigma>\<^sub>S' = (unboolify (boolify i1 \<and> boolify i2) # \<sigma>, \<pi>, s, \<omega>)" by simp
     let ?\<mu> = "stack_to_mem (i1 # i2 # \<sigma>) \<mu>"
     let ?\<Sigma>\<^sub>A\<^sub>1 = "(?\<mu>, Some (?\<mu> 0), d, 
-      [CBAssm {D} (Reg M), ABAssm 0, CBAssm {A, M} (Decr M), CBAssm {M} DOrM, ABAssm 0] @ ?\<pi>', \<omega>)"
+      [CBAssm {D} (Reg M), ABAssm 0, CBAssm {A, M} (Decr M), CBAssm {M} DAndM, ABAssm 0] @ ?\<pi>', s, \<omega>)"
     let ?\<Sigma>\<^sub>A\<^sub>2 = "(?\<mu>, Some (?\<mu> 0), ?\<mu> (?\<mu> 0), 
-      [ABAssm 0, CBAssm {A, M} (Decr M), CBAssm {M} DOrM, ABAssm 0] @ ?\<pi>', \<omega>)"
+      [ABAssm 0, CBAssm {A, M} (Decr M), CBAssm {M} DAndM, ABAssm 0] @ ?\<pi>', s, \<omega>)"
     let ?\<Sigma>\<^sub>A\<^sub>3 = "(?\<mu>, Some 0, ?\<mu> (?\<mu> 0), 
-      [CBAssm {A, M} (Decr M), CBAssm {M} DOrM, ABAssm 0] @ ?\<pi>', \<omega>)"
+      [CBAssm {A, M} (Decr M), CBAssm {M} DAndM, ABAssm 0] @ ?\<pi>', s, \<omega>)"
     let ?\<Sigma>\<^sub>A\<^sub>4 = "(?\<mu>(0 := ?\<mu> 0 - 1), Some (?\<mu> 0 - 1), ?\<mu> (?\<mu> 0), 
-      [CBAssm {M} DOrM, ABAssm 0] @ ?\<pi>', \<omega>)"
-    let ?\<Sigma>\<^sub>A\<^sub>5 = "(stack_to_mem (unboolify (boolify i1 \<or> boolify i2) # \<sigma>) ?\<mu>, Some (?\<mu> 0 - 1), 
-      ?\<mu> (?\<mu> 0), [ABAssm 0] @ ?\<pi>', \<omega>)"
-    let ?\<Sigma>\<^sub>A\<^sub>6 = "(stack_to_mem (unboolify (boolify i1 \<or> boolify i2) # \<sigma>) ?\<mu>, Some 0, 
-      ?\<mu> (?\<mu> 0), ?\<pi>', \<omega>)"
+      [CBAssm {M} DAndM, ABAssm 0] @ ?\<pi>', s, \<omega>)"
+    let ?\<Sigma>\<^sub>A\<^sub>5 = "(stack_to_mem (unboolify (boolify i1 \<and> boolify i2) # \<sigma>) ?\<mu>, Some (?\<mu> 0 - 1), 
+      ?\<mu> (?\<mu> 0), [ABAssm 0] @ ?\<pi>', s, \<omega>)"
+    let ?\<Sigma>\<^sub>A\<^sub>6 = "(stack_to_mem (unboolify (boolify i1 \<and> boolify i2) # \<sigma>) ?\<mu>, Some 0, 
+      ?\<mu> (?\<mu> 0), ?\<pi>', s, \<omega>)"
     from M have step1: "eval_b_assembly (program_convert \<Pi>) \<Sigma>\<^sub>A = Some ?\<Sigma>\<^sub>A\<^sub>1" by simp
     have step2: "eval_b_assembly (program_convert \<Pi>) ?\<Sigma>\<^sub>A\<^sub>1 = Some ?\<Sigma>\<^sub>A\<^sub>2" by simp
     have step3: "eval_b_assembly (program_convert \<Pi>) ?\<Sigma>\<^sub>A\<^sub>2 = Some ?\<Sigma>\<^sub>A\<^sub>3" by simp
@@ -451,18 +447,50 @@ lemma eval_stack_conv [simp]: "eval_stack \<Pi> \<Sigma>\<^sub>S = Some \<Sigma>
     moreover from iter_two iter_prestep step4 step5 step6 have
       "iterate (eval_b_assembly (program_convert \<Pi>)) ?\<Sigma>\<^sub>A\<^sub>3 ?\<Sigma>\<^sub>A\<^sub>6" by fast
     ultimately have X: "iterate (eval_b_assembly (program_convert \<Pi>)) \<Sigma>\<^sub>A ?\<Sigma>\<^sub>A\<^sub>6" by fast
-    have "?\<Sigma>\<^sub>A\<^sub>6 \<in> state_convert (unboolify (boolify i1 \<or> boolify i2) # \<sigma>, \<pi>, \<omega>)" by auto
+    have "?\<Sigma>\<^sub>A\<^sub>6 \<in> state_convert (unboolify (boolify i1 \<and> boolify i2) # \<sigma>, \<pi>, s, \<omega>)" by auto
     with X S M show ?case by metis
-  next case (9 \<Pi> i1 \<sigma> \<pi> \<omega>)
+  next case (9 \<Pi> i1 i2 \<sigma> \<pi> s \<omega>)
     let ?\<pi>' = "concat (map instruction_conv \<pi>)"
-    from 9 obtain d \<mu> where M: "\<Sigma>\<^sub>A = (stack_to_mem (i1 # \<sigma>) \<mu>, Some 0, d, 
-      [CBAssm {A} (Reg M), CBAssm {M} (NotR M), ABAssm 0] @ ?\<pi>', \<omega>)" by fastforce
-    from 9 have S: "\<Sigma>\<^sub>S' = (unboolify (\<not> boolify i1) # \<sigma>, \<pi>, \<omega>)" by simp
+    from 9 obtain d \<mu> where M: "\<Sigma>\<^sub>A = (stack_to_mem (i1 # i2 # \<sigma>) \<mu>, Some 0, d, 
+      [CBAssm {A} (Reg M), CBAssm {D} (Reg M), ABAssm 0, 
+       CBAssm {A, M} (Decr M), CBAssm {M} DOrM, ABAssm 0] @ ?\<pi>', s, \<omega>)" by fastforce
+    from 9 have S: "\<Sigma>\<^sub>S' = (unboolify (boolify i1 \<or> boolify i2) # \<sigma>, \<pi>, s, \<omega>)" by simp
+    let ?\<mu> = "stack_to_mem (i1 # i2 # \<sigma>) \<mu>"
+    let ?\<Sigma>\<^sub>A\<^sub>1 = "(?\<mu>, Some (?\<mu> 0), d, 
+      [CBAssm {D} (Reg M), ABAssm 0, CBAssm {A, M} (Decr M), CBAssm {M} DOrM, ABAssm 0] @ ?\<pi>', s, \<omega>)"
+    let ?\<Sigma>\<^sub>A\<^sub>2 = "(?\<mu>, Some (?\<mu> 0), ?\<mu> (?\<mu> 0), 
+      [ABAssm 0, CBAssm {A, M} (Decr M), CBAssm {M} DOrM, ABAssm 0] @ ?\<pi>', s, \<omega>)"
+    let ?\<Sigma>\<^sub>A\<^sub>3 = "(?\<mu>, Some 0, ?\<mu> (?\<mu> 0), 
+      [CBAssm {A, M} (Decr M), CBAssm {M} DOrM, ABAssm 0] @ ?\<pi>', s, \<omega>)"
+    let ?\<Sigma>\<^sub>A\<^sub>4 = "(?\<mu>(0 := ?\<mu> 0 - 1), Some (?\<mu> 0 - 1), ?\<mu> (?\<mu> 0), 
+      [CBAssm {M} DOrM, ABAssm 0] @ ?\<pi>', s, \<omega>)"
+    let ?\<Sigma>\<^sub>A\<^sub>5 = "(stack_to_mem (unboolify (boolify i1 \<or> boolify i2) # \<sigma>) ?\<mu>, Some (?\<mu> 0 - 1), 
+      ?\<mu> (?\<mu> 0), [ABAssm 0] @ ?\<pi>', s, \<omega>)"
+    let ?\<Sigma>\<^sub>A\<^sub>6 = "(stack_to_mem (unboolify (boolify i1 \<or> boolify i2) # \<sigma>) ?\<mu>, Some 0, 
+      ?\<mu> (?\<mu> 0), ?\<pi>', s, \<omega>)"
+    from M have step1: "eval_b_assembly (program_convert \<Pi>) \<Sigma>\<^sub>A = Some ?\<Sigma>\<^sub>A\<^sub>1" by simp
+    have step2: "eval_b_assembly (program_convert \<Pi>) ?\<Sigma>\<^sub>A\<^sub>1 = Some ?\<Sigma>\<^sub>A\<^sub>2" by simp
+    have step3: "eval_b_assembly (program_convert \<Pi>) ?\<Sigma>\<^sub>A\<^sub>2 = Some ?\<Sigma>\<^sub>A\<^sub>3" by simp
+    have step4: "eval_b_assembly (program_convert \<Pi>) ?\<Sigma>\<^sub>A\<^sub>3 = Some ?\<Sigma>\<^sub>A\<^sub>4" by (simp add: Let_def)
+    have step5: "eval_b_assembly (program_convert \<Pi>) ?\<Sigma>\<^sub>A\<^sub>4 = Some ?\<Sigma>\<^sub>A\<^sub>5" by simp
+    have step6: "eval_b_assembly (program_convert \<Pi>) ?\<Sigma>\<^sub>A\<^sub>5 = Some ?\<Sigma>\<^sub>A\<^sub>6" by simp
+    from iter_two iter_prestep step1 step2 step3 have
+      "iterate (eval_b_assembly (program_convert \<Pi>)) \<Sigma>\<^sub>A ?\<Sigma>\<^sub>A\<^sub>3" by fast
+    moreover from iter_two iter_prestep step4 step5 step6 have
+      "iterate (eval_b_assembly (program_convert \<Pi>)) ?\<Sigma>\<^sub>A\<^sub>3 ?\<Sigma>\<^sub>A\<^sub>6" by fast
+    ultimately have X: "iterate (eval_b_assembly (program_convert \<Pi>)) \<Sigma>\<^sub>A ?\<Sigma>\<^sub>A\<^sub>6" by fast
+    have "?\<Sigma>\<^sub>A\<^sub>6 \<in> state_convert (unboolify (boolify i1 \<or> boolify i2) # \<sigma>, \<pi>, s, \<omega>)" by auto
+    with X S M show ?case by metis
+  next case (10 \<Pi> i1 \<sigma> \<pi> s \<omega>)
+    let ?\<pi>' = "concat (map instruction_conv \<pi>)"
+    from 10 obtain d \<mu> where M: "\<Sigma>\<^sub>A = (stack_to_mem (i1 # \<sigma>) \<mu>, Some 0, d, 
+      [CBAssm {A} (Reg M), CBAssm {M} (NotR M), ABAssm 0] @ ?\<pi>', s, \<omega>)" by fastforce
+    from 10 have S: "\<Sigma>\<^sub>S' = (unboolify (\<not> boolify i1) # \<sigma>, \<pi>, s, \<omega>)" by simp
     let ?\<mu> = "stack_to_mem (i1 # \<sigma>) \<mu>"
-    let ?\<Sigma>\<^sub>A\<^sub>1 = "(?\<mu>, Some (?\<mu> 0), d, [CBAssm {M} (NotR M), ABAssm 0] @ ?\<pi>', \<omega>)"
+    let ?\<Sigma>\<^sub>A\<^sub>1 = "(?\<mu>, Some (?\<mu> 0), d, [CBAssm {M} (NotR M), ABAssm 0] @ ?\<pi>', s, \<omega>)"
     let ?\<Sigma>\<^sub>A\<^sub>2 = "(?\<mu>(?\<mu> 0 := unboolify (\<not> boolify (?\<mu> (?\<mu> 0)))), Some (?\<mu> 0), d, 
-      [ABAssm 0] @ ?\<pi>', \<omega>)"
-    let ?\<Sigma>\<^sub>A\<^sub>3 = "(?\<mu>(?\<mu> 0 := unboolify (\<not> boolify (?\<mu> (?\<mu> 0)))), Some 0, d, ?\<pi>', \<omega>)"
+      [ABAssm 0] @ ?\<pi>', s, \<omega>)"
+    let ?\<Sigma>\<^sub>A\<^sub>3 = "(?\<mu>(?\<mu> 0 := unboolify (\<not> boolify (?\<mu> (?\<mu> 0)))), Some 0, d, ?\<pi>', s, \<omega>)"
     from M have step1: "eval_b_assembly (program_convert \<Pi>) \<Sigma>\<^sub>A = Some ?\<Sigma>\<^sub>A\<^sub>1" by simp
     have step2: "eval_b_assembly (program_convert \<Pi>) ?\<Sigma>\<^sub>A\<^sub>1 = Some ?\<Sigma>\<^sub>A\<^sub>2" by simp
     have "eval_b_assembly (program_convert \<Pi>) ?\<Sigma>\<^sub>A\<^sub>2 = Some ?\<Sigma>\<^sub>A\<^sub>3" by simp
@@ -470,21 +498,22 @@ lemma eval_stack_conv [simp]: "eval_stack \<Pi> \<Sigma>\<^sub>S = Some \<Sigma>
       "iterate (eval_b_assembly (program_convert \<Pi>)) \<Sigma>\<^sub>A ?\<Sigma>\<^sub>A\<^sub>3" by fast
     have "(stack_to_mem (i1 # \<sigma>) \<mu>)(1 + int (length \<sigma>) := unboolify (\<not> boolify i1)) = 
       stack_to_mem (unboolify (\<not> boolify i1) # \<sigma>) \<mu>" by auto
-    hence "?\<Sigma>\<^sub>A\<^sub>3 \<in> state_convert (unboolify (\<not> boolify i1) # \<sigma>, \<pi>, \<omega>)" by auto
+    hence "?\<Sigma>\<^sub>A\<^sub>3 \<in> state_convert (unboolify (\<not> boolify i1) # \<sigma>, \<pi>, s, \<omega>)" by auto
     with X S M show ?case by metis
-  next case (10 \<Pi> i1 \<sigma> \<pi> \<omega>)
+  next case (11 \<Pi> i1 \<sigma> \<pi> s \<omega>)
     let ?\<pi>' = "concat (map instruction_conv \<pi>)"
-    from 10 have S: "\<Sigma>\<^sub>S' = (\<sigma>, \<pi>, i1 # \<omega>)" by simp
-    from 10 obtain d \<mu> where M: "\<Sigma>\<^sub>A = (stack_to_mem (i1 # \<sigma>) \<mu>, Some 0, d, 
-        [CBAssm {A} (Reg M), CBAssm {D} (Reg M), PBAssm, ABAssm 0, CBAssm {M} (Decr M)] @ ?\<pi>', \<omega>)" 
+    from 11 have S: "\<Sigma>\<^sub>S' = (\<sigma>, \<pi>, s, i1 # \<omega>)" by simp
+    from 11 obtain d \<mu> where M: "\<Sigma>\<^sub>A = (stack_to_mem (i1 # \<sigma>) \<mu>, Some 0, d, 
+        [CBAssm {A} (Reg M), CBAssm {D} (Reg M), PBAssm, ABAssm 0, CBAssm {M} (Decr M)] @ ?\<pi>', s, \<omega>)" 
       by fastforce
     let ?\<mu> = "stack_to_mem (i1 # \<sigma>) \<mu>"
     let ?\<Sigma>\<^sub>A\<^sub>1 = "(?\<mu>, Some (?\<mu> 0), d, 
-      [CBAssm {D} (Reg M), PBAssm, ABAssm 0, CBAssm {M} (Decr M)] @ ?\<pi>', \<omega>)"
-    let ?\<Sigma>\<^sub>A\<^sub>2 = "(?\<mu>, Some (?\<mu> 0), ?\<mu> (?\<mu> 0), [PBAssm, ABAssm 0, CBAssm {M} (Decr M)] @ ?\<pi>', \<omega>)"
-    let ?\<Sigma>\<^sub>A\<^sub>3 = "(?\<mu>, Some (?\<mu> 0), ?\<mu> (?\<mu> 0), [ABAssm 0, CBAssm {M} (Decr M)] @ ?\<pi>', ?\<mu> (?\<mu> 0) # \<omega>)"
-    let ?\<Sigma>\<^sub>A\<^sub>4 = "(?\<mu>, Some 0, ?\<mu> (?\<mu> 0), [CBAssm {M} (Decr M)] @ ?\<pi>', ?\<mu> (?\<mu> 0) # \<omega>)"
-    let ?\<Sigma>\<^sub>A\<^sub>5 = "(?\<mu>(0 := ?\<mu> 0 - 1), Some 0, ?\<mu> (?\<mu> 0), ?\<pi>', ?\<mu> (?\<mu> 0) # \<omega>)"
+      [CBAssm {D} (Reg M), PBAssm, ABAssm 0, CBAssm {M} (Decr M)] @ ?\<pi>', s, \<omega>)"
+    let ?\<Sigma>\<^sub>A\<^sub>2 = "(?\<mu>, Some (?\<mu> 0), ?\<mu> (?\<mu> 0), [PBAssm, ABAssm 0, CBAssm {M} (Decr M)] @ ?\<pi>', s, \<omega>)"
+    let ?\<Sigma>\<^sub>A\<^sub>3 = "(?\<mu>, Some (?\<mu> 0), ?\<mu> (?\<mu> 0), 
+      [ABAssm 0, CBAssm {M} (Decr M)] @ ?\<pi>', s, ?\<mu> (?\<mu> 0) # \<omega>)"
+    let ?\<Sigma>\<^sub>A\<^sub>4 = "(?\<mu>, Some 0, ?\<mu> (?\<mu> 0), [CBAssm {M} (Decr M)] @ ?\<pi>', s, ?\<mu> (?\<mu> 0) # \<omega>)"
+    let ?\<Sigma>\<^sub>A\<^sub>5 = "(?\<mu>(0 := ?\<mu> 0 - 1), Some 0, ?\<mu> (?\<mu> 0), ?\<pi>', s, ?\<mu> (?\<mu> 0) # \<omega>)"
     from M have step1: "eval_b_assembly (program_convert \<Pi>) \<Sigma>\<^sub>A = Some ?\<Sigma>\<^sub>A\<^sub>1" by simp
     have step2: "eval_b_assembly (program_convert \<Pi>) ?\<Sigma>\<^sub>A\<^sub>1 = Some ?\<Sigma>\<^sub>A\<^sub>2" by simp
     have step3: "eval_b_assembly (program_convert \<Pi>) ?\<Sigma>\<^sub>A\<^sub>2 = Some ?\<Sigma>\<^sub>A\<^sub>3" by simp
@@ -495,36 +524,34 @@ lemma eval_stack_conv [simp]: "eval_stack \<Pi> \<Sigma>\<^sub>S = Some \<Sigma>
     moreover from iter_two step4 step5 have 
       "iterate (eval_b_assembly (program_convert \<Pi>)) ?\<Sigma>\<^sub>A\<^sub>3 ?\<Sigma>\<^sub>A\<^sub>5" by fast
     ultimately have X: "iterate (eval_b_assembly (program_convert \<Pi>)) \<Sigma>\<^sub>A ?\<Sigma>\<^sub>A\<^sub>5" by fast
-    have "?\<Sigma>\<^sub>A\<^sub>5 \<in> state_convert (\<sigma>, \<pi>, i1 # \<omega>)" by auto
+    have "?\<Sigma>\<^sub>A\<^sub>5 \<in> state_convert (\<sigma>, \<pi>, s, i1 # \<omega>)" by auto
     with X S M show ?case by metis
   next
 
   (* autogenerated cases where "eval_stack \<Pi> \<Sigma>\<^sub>S = None" *)
-  case "11_1" thus ?case by simp
-  next case "11_2" thus ?case by simp
-  next case "11_3" thus ?case by simp
-  next case "11_4" thus ?case by simp
-  next case "11_5" thus ?case by simp
-  next case "11_6" thus ?case by simp
-  next case "11_7" thus ?case by simp
-  next case "11_8" thus ?case by simp
-  next case "11_9" thus ?case by simp
-  next case "11_10" thus ?case by simp
-  next case "11_11" thus ?case by simp
-  next case "11_12" thus ?case by simp
-  next case "11_13" thus ?case by simp
-  next case "11_14" thus ?case by simp
-  next case "11_15" thus ?case by simp
-  next case "11_16" thus ?case by simp
-  next case "11_17" thus ?case by simp
-  next case "11_18" thus ?case by simp
-  next case "11_19" thus ?case by simp
-  next case "11_20" thus ?case by simp
-  next case "11_21" thus ?case by simp
-  next case "11_22" thus ?case by simp
-  next case "11_23" thus ?case by simp
-  next case "11_24" thus ?case by simp
-  next case "11_25" thus ?case by simp
+  case "12_1" thus ?case by simp
+  next case "12_2" thus ?case by simp
+  next case "12_3" thus ?case by simp
+  next case "12_4" thus ?case by simp
+  next case "12_5" thus ?case by simp
+  next case "12_6" thus ?case by simp
+  next case "12_7" thus ?case by simp
+  next case "12_8" thus ?case by simp
+  next case "12_9" thus ?case by simp
+  next case "12_10" thus ?case by simp
+  next case "12_11" thus ?case by simp
+  next case "12_12" thus ?case by simp
+  next case "12_13" thus ?case by simp
+  next case "12_14" thus ?case by simp
+  next case "12_15" thus ?case by simp
+  next case "12_16" thus ?case by simp
+  next case "12_17" thus ?case by simp
+  next case "12_18" thus ?case by simp
+  next case "12_19" thus ?case by simp
+  next case "12_20" thus ?case by simp
+  next case "12_21" thus ?case by simp
+  next case "12_22" thus ?case by simp
+  next case "12_23" thus ?case by simp
   qed
 
 theorem stack_to_assembly_correct [simp]: "iterate (eval_stack \<Pi>) \<Sigma>\<^sub>S \<Sigma>\<^sub>S' \<Longrightarrow> 
