LinearAssemblyLanguage.thy
@@ -2,9 +2,12 @@ theory LinearAssemblyLanguage
 imports AssemblyLanguage FiniteMap Iterate
 begin
 
+type_synonym l_assembly_state = "memory \<times> int option \<times> int \<times> assembly list \<times> output" 
+  (* \<mu>, a, d, \<pi>, \<omega> *)
+
 type_synonym l_assembly_program = "code_label \<leadsto> assembly list"
 
-fun eval_l_assembly :: "l_assembly_program \<Rightarrow> assembly_state \<Rightarrow> assembly_state option" where
+fun eval_l_assembly :: "l_assembly_program \<Rightarrow> l_assembly_state \<Rightarrow> l_assembly_state option" where
   "eval_l_assembly \<Pi> (\<mu>, a, d, [], \<omega>) = None"
 | "eval_l_assembly \<Pi> (\<mu>, a, d, AAssm x # \<pi>, \<omega>) = Some (\<mu>, Some x, d, \<pi>, \<omega>)"
 | "eval_l_assembly \<Pi> (\<mu>, Some a, d, CAssm dst cmp # \<pi>, \<omega>) = (
@@ -13,8 +16,7 @@ fun eval_l_assembly :: "l_assembly_program \<Rightarrow> assembly_state \<Righta
       if M \<in> dst then \<mu>(a := n) else \<mu>, 
       Some (if A \<in> dst then n else a), 
       if D \<in> dst then n else d, 
-      \<pi>, 
-      \<omega>))"
+      \<pi>, \<omega>))"
 | "eval_l_assembly \<Pi> (\<mu>, None, d, CAssm dst cmp # \<pi>, \<omega>) = None"
 | "eval_l_assembly \<Pi> (\<mu>, a, d, JAssm jmp s # \<pi>, \<omega>) = (
     if should_jump d jmp
@@ -28,20 +30,7 @@ fun eval_l_assembly :: "l_assembly_program \<Rightarrow> assembly_state \<Righta
 
 lemma [simp]: "finite (dom \<Pi>) \<Longrightarrow> eval_assembly \<Pi> \<Sigma> = Some \<Sigma>' \<Longrightarrow> 
     eval_l_assembly (linearize \<Pi>) \<Sigma> = Some \<Sigma>'"
-  proof (induction \<Pi> \<Sigma> rule: eval_assembly.induct)
-  case 1
-    from 1(2) show ?case by simp
-  next case 2
-    thus ?case by simp
-  next case 3
-    thus ?case by simp
-  next case 4
-    from 4(2) show ?case by simp
-  next case 5
-    thus ?case by auto
-  next case 6
-    thus ?case by simp
-  qed 
+  by (induction \<Pi> \<Sigma> rule: eval_assembly.induct) auto
 
 theorem linearization_correct [simp]: "iterate (eval_assembly \<Pi>) \<Sigma> \<Sigma>' \<Longrightarrow> finite (dom \<Pi>) \<Longrightarrow> 
     iterate (eval_l_assembly (linearize \<Pi>)) \<Sigma> \<Sigma>'"
